<?xml version="1.0"?>
<rdf:RDF xmlns="http://purl.obolibrary.org/obo/uber-gpo.owl#"
     xml:base="http://purl.obolibrary.org/obo/uber-gpo.owl"
     xmlns:obo="http://purl.obolibrary.org/obo/"
     xmlns:rdfs="http://www.w3.org/2000/01/rdf-schema#"
     xmlns:owl="http://www.w3.org/2002/07/owl#"
     xmlns:xsd="http://www.w3.org/2001/XMLSchema#"
     xmlns:rdf="http://www.w3.org/1999/02/22-rdf-syntax-ns#">
    <owl:Ontology rdf:about="http://purl.obolibrary.org/obo/mgpo.owl">
        <rdfs:comment>This initial draft presents a hierarchy of molecular glyco-phenotype classes, and is intended to demonstrate the utility of different axes by which to structure the ontology.  It will be used to get feedback on definitions, granularity, and classification from domain experts and ontologists.

This in turn will inform implementation of upstream modeling in orthogonal ontologies (ChEBI, GO,PATO), that will be used to (semi)-automate the generation of the mgpo module as part of a larger Causal Phenotype Netrok approach described here: https://code.google.com/p/phenotype-ontologies/source/browse/trunk/src/ontology/cpn/causal-pheno-networks.md.


</rdfs:comment>
    </owl:Ontology>
    


    <!-- 
    ///////////////////////////////////////////////////////////////////////////////////////
    //
    // Annotation properties
    //
    ///////////////////////////////////////////////////////////////////////////////////////
     -->

    


    <!-- http://purl.obolibrary.org/obo/IAO_0000115 -->

    <owl:AnnotationProperty rdf:about="http://purl.obolibrary.org/obo/IAO_0000115">
        <rdfs:label xml:lang="en">definition</rdfs:label>
    </owl:AnnotationProperty>
    


    <!-- http://purl.obolibrary.org/obo/UPHENO_0002032 -->

    <owl:AnnotationProperty rdf:about="http://purl.obolibrary.org/obo/UPHENO_0002032">
        <rdfs:label xml:lang="en">mgpo_editor_note</rdfs:label>
    </owl:AnnotationProperty>
    


    <!-- http://purl.obolibrary.org/obo/UPHENO_0002037 -->

    <owl:AnnotationProperty rdf:about="http://purl.obolibrary.org/obo/UPHENO_0002037">
        <rdfs:label xml:lang="en">alternative term</rdfs:label>
    </owl:AnnotationProperty>
    


    <!-- 
    ///////////////////////////////////////////////////////////////////////////////////////
    //
    // Classes
    //
    ///////////////////////////////////////////////////////////////////////////////////////
     -->

    


    <!-- http://purl.obolibrary.org/obo/UPHENO_0001001 -->

    <owl:Class rdf:about="http://purl.obolibrary.org/obo/UPHENO_0001001">
        <rdfs:label xml:lang="en">Phenotype</rdfs:label>
    </owl:Class>
    


    <!-- http://purl.obolibrary.org/obo/UPHENO_0002001 -->

    <owl:Class rdf:about="http://purl.obolibrary.org/obo/UPHENO_0002001">
        <rdfs:label xml:lang="en">abnormal glycan metabolism</rdfs:label>
        <rdfs:subClassOf rdf:resource="http://purl.obolibrary.org/obo/UPHENO_0002005"/>
        <obo:IAO_0000115>An abnormality in the process of glycan catabolism or biosynthesis.</obo:IAO_0000115>
    </owl:Class>
    


    <!-- http://purl.obolibrary.org/obo/UPHENO_0002002 -->

    <owl:Class rdf:about="http://purl.obolibrary.org/obo/UPHENO_0002002">
        <rdfs:label xml:lang="en">abnormal glycan level</rdfs:label>
        <rdfs:subClassOf rdf:resource="http://purl.obolibrary.org/obo/UPHENO_0002033"/>
        <rdfs:comment>The distinction between abnormal glycan levels and abnormal glycan structure/composition is confounded by the fact that specific phenotypes in both categories are typically reported in the literature by describing  the amount of a particular type of glycan. For example, &quot;increased sialylated oligosaccharides in the lysosome&quot; is verbatim text reporting a ‘compositional’ defect, and &quot;increased levels of complex N-Glycans in the serum&quot;  is verbatim text reporting a ‘level’ defect. The key difference is that the former defect indicates that glycans contain abnormalities in their sialyl content that make them compositionally different that glycan end products normally found in the lysosome. And biologically, this defect likely results from defects in glycosylation, deglycosylation, or isomerase enzymes.  By contrast, the latter defect does not reflect a structural/compositional abnormality in the specified glycan, but rather that the level of a certain normal type of glycan end-product is elevated. Compared to a compositional phenotype, this defect likely has a very different biological cause related to abnormal glycan degradation or trafficking.</rdfs:comment>
        <obo:IAO_0000115>An increase or decrease in the amount or concentration of normal gycan structures present in the body, cell, or specific location therein.</obo:IAO_0000115>
    </owl:Class>
    


    <!-- http://purl.obolibrary.org/obo/UPHENO_0002003 -->

    <owl:Class rdf:about="http://purl.obolibrary.org/obo/UPHENO_0002003">
        <rdfs:label xml:lang="en">abnormal glycan occupancy</rdfs:label>
        <rdfs:subClassOf rdf:resource="http://purl.obolibrary.org/obo/UPHENO_0002033"/>
        <rdfs:comment>&quot;Occupancy&quot; is used here to describe the extent of conjugation of a glycan chain to glycosylation sites on an aglycone target. Abnormal occupancy does not speak to the structure or composition of the glycan chain, just the relative abundance of glycan chains on some protein or lipid target.</rdfs:comment>
        <obo:UPHENO_0002032>Relevant Classification Axes (in order shown for exemplar classes below):
1  glycosylation/target type (N-linked vs O-linked vs proteoglycan)
1.1  glycosylated residue (e.g. Asn, Ser, Thr)
1.2  specific aglycone target (e.g. transferrin)
1.2.1  anatomical/cellular location (e.g. serum, golgi)
</obo:UPHENO_0002032>
        <obo:IAO_0000115>An increase or decrease in the number of glycan chains conjugated to an aglycone target.</obo:IAO_0000115>
    </owl:Class>
    


    <!-- http://purl.obolibrary.org/obo/UPHENO_0002004 -->

    <owl:Class rdf:about="http://purl.obolibrary.org/obo/UPHENO_0002004">
        <rdfs:label xml:lang="en">abnormal glycan structure</rdfs:label>
        <rdfs:subClassOf rdf:resource="http://purl.obolibrary.org/obo/UPHENO_0002033"/>
        <rdfs:comment>A change in the molecular structure of a glycan, including altered sugar composition, chain length, linkage or branching patterns, or modifications on a sugar residues</rdfs:comment>
        <rdfs:comment>The distinction between abnormal glycan levels and abnormal glycan structure/composition is confounded by the fact that specific phenotypes in both categories are typically reported in the literature by describing  the amount of a particular type of glycan. For example, &quot;increased sialylated oligosaccharides in the lysosome&quot; is verbatim text reporting a ‘compositional’ defect, and &quot;increased levels of complex N-Glycans in the serum&quot;  is verbatim text reporting a ‘level’ defect. The key difference is that the former defect indicates that glycans contain abnormalities in their sialyl content that make them compositionally different that glycan end products normally found in the lysosome. And biologically, this defect likely results from defects in glycosylation, deglycosylation, or isomerase enzymes.  By contrast, the latter defect does not reflect a structural/compositional abnormality in the specified glycan, but rather that the level of a certain normal type of glycan end-product is elevated. Compared to a compositional phenotype, this defect likely has a very different biological cause related to abnormal glycan degradation or trafficking.</rdfs:comment>
    </owl:Class>
    


    <!-- http://purl.obolibrary.org/obo/UPHENO_0002005 -->

    <owl:Class rdf:about="http://purl.obolibrary.org/obo/UPHENO_0002005">
        <rdfs:label xml:lang="en">abnormal process phenotype</rdfs:label>
        <rdfs:subClassOf rdf:resource="http://purl.obolibrary.org/obo/UPHENO_0001001"/>
        <obo:IAO_0000115>Abnormality in a biological process.</obo:IAO_0000115>
    </owl:Class>
    


    <!-- http://purl.obolibrary.org/obo/UPHENO_0002006 -->

    <owl:Class rdf:about="http://purl.obolibrary.org/obo/UPHENO_0002006">
        <rdfs:label xml:lang="en">abnormal glycan binding</rdfs:label>
        <rdfs:subClassOf rdf:resource="http://purl.obolibrary.org/obo/UPHENO_0002005"/>
        <obo:IAO_0000115>An abnormality in the process of a glycan binding to its target.</obo:IAO_0000115>
    </owl:Class>
    


    <!-- http://purl.obolibrary.org/obo/UPHENO_0002007 -->

    <owl:Class rdf:about="http://purl.obolibrary.org/obo/UPHENO_0002007">
        <rdfs:label xml:lang="en">abnormal deglycosylation</rdfs:label>
        <rdfs:subClassOf rdf:resource="http://purl.obolibrary.org/obo/UPHENO_0002005"/>
        <obo:IAO_0000115>An abnormality in the process of glycan deglycosylation.</obo:IAO_0000115>
    </owl:Class>
    


    <!-- http://purl.obolibrary.org/obo/UPHENO_0002008 -->

    <owl:Class rdf:about="http://purl.obolibrary.org/obo/UPHENO_0002008">
        <rdfs:label xml:lang="en">abnormal glycan catabolism</rdfs:label>
        <rdfs:subClassOf rdf:resource="http://purl.obolibrary.org/obo/UPHENO_0002001"/>
    </owl:Class>
    


    <!-- http://purl.obolibrary.org/obo/UPHENO_0002009 -->

    <owl:Class rdf:about="http://purl.obolibrary.org/obo/UPHENO_0002009">
        <rdfs:label xml:lang="en">abnormal glycosylation</rdfs:label>
        <rdfs:subClassOf rdf:resource="http://purl.obolibrary.org/obo/UPHENO_0002030"/>
    </owl:Class>
    


    <!-- http://purl.obolibrary.org/obo/UPHENO_0002010 -->

    <owl:Class rdf:about="http://purl.obolibrary.org/obo/UPHENO_0002010">
        <rdfs:label xml:lang="en">abnormal glycan branching</rdfs:label>
        <rdfs:subClassOf rdf:resource="http://purl.obolibrary.org/obo/UPHENO_0002004"/>
        <obo:UPHENO_0002032>Relevant Classification Axes (in order shown for exemplar classes above):
1  attachment (conjugated vs free glycans)
1.1  aglycone class (e.g. glycoprotein-linked vs glycopeptide-linked)
1.1.1  more specific aglycone class (e.g. N-glycan  vs O-glycan for proteins)
</obo:UPHENO_0002032>
        <obo:IAO_0000115>A change in the structure of a glycan chain due to altered branching patterns. </obo:IAO_0000115>
    </owl:Class>
    


    <!-- http://purl.obolibrary.org/obo/UPHENO_0002011 -->

    <owl:Class rdf:about="http://purl.obolibrary.org/obo/UPHENO_0002011">
        <rdfs:label xml:lang="en">abnormal glycan composition</rdfs:label>
        <rdfs:subClassOf rdf:resource="http://purl.obolibrary.org/obo/UPHENO_0002004"/>
        <obo:UPHENO_0002037>abnormal glycan chain composition</obo:UPHENO_0002037>
        <obo:IAO_0000115>A change in the strucutre of a glycan chain due to variations in number and/or type of sugar residue constituents - typically an increased or decreased abundance of a given type of residue, or the substitution of on residue type for another.</obo:IAO_0000115>
    </owl:Class>
    


    <!-- http://purl.obolibrary.org/obo/UPHENO_0002012 -->

    <owl:Class rdf:about="http://purl.obolibrary.org/obo/UPHENO_0002012">
        <rdfs:label xml:lang="en">abnormal N-linked glycoprotein occupancy</rdfs:label>
        <rdfs:subClassOf rdf:resource="http://purl.obolibrary.org/obo/UPHENO_0002003"/>
        <obo:IAO_0000115>An increase or decrease in the number of N-glycan chains conjugated to aglycone targets.</obo:IAO_0000115>
    </owl:Class>
    


    <!-- http://purl.obolibrary.org/obo/UPHENO_0002013 -->

    <owl:Class rdf:about="http://purl.obolibrary.org/obo/UPHENO_0002013">
        <rdfs:label xml:lang="en">abnormal O-linked glycoprotein occupancy</rdfs:label>
        <rdfs:subClassOf rdf:resource="http://purl.obolibrary.org/obo/UPHENO_0002003"/>
        <obo:IAO_0000115>An increase or decrease in the number of O-glycan chains conjugated to aglycone targets.</obo:IAO_0000115>
    </owl:Class>
    


    <!-- http://purl.obolibrary.org/obo/UPHENO_0002014 -->

    <owl:Class rdf:about="http://purl.obolibrary.org/obo/UPHENO_0002014">
        <rdfs:label xml:lang="en">abnormal N-glycan levels</rdfs:label>
        <rdfs:subClassOf rdf:resource="http://purl.obolibrary.org/obo/UPHENO_0002077"/>
        <obo:IAO_0000115>An increase or decrease in the amount or concentration of normal N-gycan structures present in the body, cell, or specific location therein.</obo:IAO_0000115>
    </owl:Class>
    


    <!-- http://purl.obolibrary.org/obo/UPHENO_0002015 -->

    <owl:Class rdf:about="http://purl.obolibrary.org/obo/UPHENO_0002015">
        <rdfs:label xml:lang="en">abnormal O-glycan levels</rdfs:label>
        <rdfs:subClassOf rdf:resource="http://purl.obolibrary.org/obo/UPHENO_0002077"/>
        <obo:IAO_0000115>An increase or decrease in the amount or concentration of normal O-gycan structures present in the body, cell, or specific location therein.</obo:IAO_0000115>
    </owl:Class>
    


    <!-- http://purl.obolibrary.org/obo/UPHENO_0002017 -->

    <owl:Class rdf:about="http://purl.obolibrary.org/obo/UPHENO_0002017">
        <rdfs:label xml:lang="en">abnormal IDUA activity</rdfs:label>
        <rdfs:subClassOf rdf:resource="http://purl.obolibrary.org/obo/UPHENO_0002036"/>
        <obo:IAO_0000115>Altered IDUA enzymatic activity in an organism, cell, or part thereof.</obo:IAO_0000115>
    </owl:Class>
    


    <!-- http://purl.obolibrary.org/obo/UPHENO_0002018 -->

    <owl:Class rdf:about="http://purl.obolibrary.org/obo/UPHENO_0002018">
        <rdfs:label xml:lang="en">abnormal heparan sulfate degradation</rdfs:label>
        <rdfs:subClassOf rdf:resource="http://purl.obolibrary.org/obo/UPHENO_0002008"/>
    </owl:Class>
    


    <!-- http://purl.obolibrary.org/obo/UPHENO_0002019 -->

    <owl:Class rdf:about="http://purl.obolibrary.org/obo/UPHENO_0002019">
        <rdfs:label xml:lang="en">abnormal R-type lectin binding</rdfs:label>
        <rdfs:subClassOf rdf:resource="http://purl.obolibrary.org/obo/UPHENO_0002006"/>
    </owl:Class>
    


    <!-- http://purl.obolibrary.org/obo/UPHENO_0002020 -->

    <owl:Class rdf:about="http://purl.obolibrary.org/obo/UPHENO_0002020">
        <rdfs:label xml:lang="en">abnormal N-glycan composition</rdfs:label>
        <rdfs:subClassOf rdf:resource="http://purl.obolibrary.org/obo/UPHENO_0002044"/>
        <obo:IAO_0000115>A change in the strucutre of an N-glycan chain due to variations in number and/or type of sugar residue constituents - typically an increased or decreased abundance of a given type of residue, or the substitution of on residue type for another.</obo:IAO_0000115>
    </owl:Class>
    


    <!-- http://purl.obolibrary.org/obo/UPHENO_0002021 -->

    <owl:Class rdf:about="http://purl.obolibrary.org/obo/UPHENO_0002021">
        <rdfs:label xml:lang="en">abnormal sialyl content in N-glycans</rdfs:label>
        <rdfs:subClassOf rdf:resource="http://purl.obolibrary.org/obo/UPHENO_0002020"/>
        <obo:IAO_0000115>A change in the strucutre of an N-glycan chain due to variations in number and/or location of sialyl residues - typically an increased or decreased abundance of sialyl residues, or the substitution of sialyl residues for another residue type.</obo:IAO_0000115>
    </owl:Class>
    


    <!-- http://purl.obolibrary.org/obo/UPHENO_0002022 -->

    <owl:Class rdf:about="http://purl.obolibrary.org/obo/UPHENO_0002022">
        <rdfs:label xml:lang="en">abnormal N-glycan branching</rdfs:label>
        <rdfs:subClassOf rdf:resource="http://purl.obolibrary.org/obo/UPHENO_0002066"/>
        <obo:IAO_0000115>A change in the structure of an N-glycan chain due to altered branching patterns. </obo:IAO_0000115>
    </owl:Class>
    


    <!-- http://purl.obolibrary.org/obo/UPHENO_0002023 -->

    <owl:Class rdf:about="http://purl.obolibrary.org/obo/UPHENO_0002023">
        <rdfs:label xml:lang="en">abnormal transferrin N-glycan occupancy</rdfs:label>
        <rdfs:subClassOf rdf:resource="http://purl.obolibrary.org/obo/UPHENO_0002012"/>
        <obo:IAO_0000115>An increase or decrease in the number of N-glycan chains conjugated to transferrin protein.</obo:IAO_0000115>
    </owl:Class>
    


    <!-- http://purl.obolibrary.org/obo/UPHENO_0002024 -->

    <owl:Class rdf:about="http://purl.obolibrary.org/obo/UPHENO_0002024">
        <rdfs:label xml:lang="en">abnormal serum transferrin N-glycan occupancy</rdfs:label>
        <rdfs:subClassOf rdf:resource="http://purl.obolibrary.org/obo/UPHENO_0002023"/>
        <obo:IAO_0000115>An increase or decrease in the number of N-glycan chains conjugated to transferrin protein in blood serum.</obo:IAO_0000115>
    </owl:Class>
    


    <!-- http://purl.obolibrary.org/obo/UPHENO_0002025 -->

    <owl:Class rdf:about="http://purl.obolibrary.org/obo/UPHENO_0002025">
        <rdfs:label xml:lang="en">abnormal complex N-glycan levels</rdfs:label>
        <rdfs:subClassOf rdf:resource="http://purl.obolibrary.org/obo/UPHENO_0002014"/>
        <obo:IAO_0000115>An increase or decrease in the amount or concentration of normal complex N-gycan structures present in the body, cell, or specific location therein.</obo:IAO_0000115>
    </owl:Class>
    


    <!-- http://purl.obolibrary.org/obo/UPHENO_0002026 -->

    <owl:Class rdf:about="http://purl.obolibrary.org/obo/UPHENO_0002026">
        <rdfs:label xml:lang="en">abnormal biantennary N-glycan levels</rdfs:label>
        <rdfs:subClassOf rdf:resource="http://purl.obolibrary.org/obo/UPHENO_0002025"/>
        <obo:IAO_0000115>An increase or decrease in the amount or concentration of normal biantennary N-gycan structures present in the body, cell, or specific location therein.</obo:IAO_0000115>
    </owl:Class>
    


    <!-- http://purl.obolibrary.org/obo/UPHENO_0002027 -->

    <owl:Class rdf:about="http://purl.obolibrary.org/obo/UPHENO_0002027">
        <rdfs:label xml:lang="en">abnormal golgi biantennary N-glycan levels</rdfs:label>
        <rdfs:subClassOf rdf:resource="http://purl.obolibrary.org/obo/UPHENO_0002026"/>
        <obo:IAO_0000115>An increase or decrease in the amount or concentration of normal biantennary N-gycan structures present in the golgi complex.</obo:IAO_0000115>
    </owl:Class>
    


    <!-- http://purl.obolibrary.org/obo/UPHENO_0002028 -->

    <owl:Class rdf:about="http://purl.obolibrary.org/obo/UPHENO_0002028">
        <rdfs:label xml:lang="en">DeprecatedClass</rdfs:label>
        <rdfs:subClassOf rdf:resource="http://purl.obolibrary.org/obo/UPHENO_0001001"/>
    </owl:Class>
    


    <!-- http://purl.obolibrary.org/obo/UPHENO_0002029 -->

    <owl:Class rdf:about="http://purl.obolibrary.org/obo/UPHENO_0002029">
        <rdfs:label xml:lang="en">abnormal activity phenotype</rdfs:label>
        <rdfs:subClassOf rdf:resource="http://purl.obolibrary.org/obo/UPHENO_0001001"/>
        <obo:IAO_0000115>An alteration in the activity of a molecular entity such as an enzyme or transporter protein</obo:IAO_0000115>
    </owl:Class>
    


    <!-- http://purl.obolibrary.org/obo/UPHENO_0002030 -->

    <owl:Class rdf:about="http://purl.obolibrary.org/obo/UPHENO_0002030">
        <rdfs:label xml:lang="en">abnormal glycan biosynthesis</rdfs:label>
        <rdfs:subClassOf rdf:resource="http://purl.obolibrary.org/obo/UPHENO_0002001"/>
    </owl:Class>
    


    <!-- http://purl.obolibrary.org/obo/UPHENO_0002031 -->

    <owl:Class rdf:about="http://purl.obolibrary.org/obo/UPHENO_0002031">
        <rdfs:label xml:lang="en">abnormal glycosaminoglycan degradation</rdfs:label>
        <rdfs:subClassOf rdf:resource="http://purl.obolibrary.org/obo/UPHENO_0002008"/>
    </owl:Class>
    


    <!-- http://purl.obolibrary.org/obo/UPHENO_0002033 -->

    <owl:Class rdf:about="http://purl.obolibrary.org/obo/UPHENO_0002033">
        <rdfs:label xml:lang="en">abnormal glycan phenotype</rdfs:label>
        <rdfs:subClassOf rdf:resource="http://purl.obolibrary.org/obo/UPHENO_0001001"/>
    </owl:Class>
    


    <!-- http://purl.obolibrary.org/obo/UPHENO_0002034 -->

    <owl:Class rdf:about="http://purl.obolibrary.org/obo/UPHENO_0002034">
        <rdfs:label xml:lang="en">abnormal glycosaminoglycan levels</rdfs:label>
        <rdfs:subClassOf rdf:resource="http://purl.obolibrary.org/obo/UPHENO_0002077"/>
        <obo:IAO_0000115>An increase or decrease in the amount or concentration of normal glycosaminoglycan gycan structures present in the body, cell, or specific location therein.</obo:IAO_0000115>
    </owl:Class>
    


    <!-- http://purl.obolibrary.org/obo/UPHENO_0002035 -->

    <owl:Class rdf:about="http://purl.obolibrary.org/obo/UPHENO_0002035">
        <rdfs:label xml:lang="en">abnormal glycosyltransferase activity</rdfs:label>
        <rdfs:subClassOf rdf:resource="http://purl.obolibrary.org/obo/UPHENO_0002029"/>
        <obo:IAO_0000115>Altered glycosyltransferase activity in an organism, cell, or part thereof.</obo:IAO_0000115>
    </owl:Class>
    


    <!-- http://purl.obolibrary.org/obo/UPHENO_0002036 -->

    <owl:Class rdf:about="http://purl.obolibrary.org/obo/UPHENO_0002036">
        <rdfs:label>abnormal glycosidase activity</rdfs:label>
        <rdfs:subClassOf rdf:resource="http://purl.obolibrary.org/obo/UPHENO_0002029"/>
        <obo:IAO_0000115>Altered glycosidase enzymatic activity in an organism, cell, or part thereof.</obo:IAO_0000115>
        <obo:UPHENO_0002037 xml:lang="en">abnormal glycosyl-hydrolase activity</obo:UPHENO_0002037>
    </owl:Class>
    


    <!-- http://purl.obolibrary.org/obo/UPHENO_0002038 -->

    <owl:Class rdf:about="http://purl.obolibrary.org/obo/UPHENO_0002038">
        <rdfs:label xml:lang="en">abnormal proteoglycan occupancy</rdfs:label>
        <rdfs:subClassOf rdf:resource="http://purl.obolibrary.org/obo/UPHENO_0002003"/>
        <obo:IAO_0000115>An increase or decrease in the extent of number of glycan chains conjugated to proteoglycans.</obo:IAO_0000115>
    </owl:Class>
    


    <!-- http://purl.obolibrary.org/obo/UPHENO_0002039 -->

    <owl:Class rdf:about="http://purl.obolibrary.org/obo/UPHENO_0002039">
        <rdfs:label xml:lang="en">abnormal N-linked glycoprotein asparagine occupancy</rdfs:label>
        <rdfs:subClassOf rdf:resource="http://purl.obolibrary.org/obo/UPHENO_0002012"/>
        <obo:IAO_0000115>An increase or decrease in the number of N-glycan chains conjugated to asparagine residues on aglycone targets.</obo:IAO_0000115>
    </owl:Class>
    


    <!-- http://purl.obolibrary.org/obo/UPHENO_0002041 -->

    <owl:Class rdf:about="http://purl.obolibrary.org/obo/UPHENO_0002041">
        <rdfs:label xml:lang="en">abnormal glycan length</rdfs:label>
        <rdfs:subClassOf rdf:resource="http://purl.obolibrary.org/obo/UPHENO_0002011"/>
        <obo:UPHENO_0002032>Relevant Classification Axes (in order shown for exemplar classes above):
1  attachment (conjugated vs free glycans)
1.1  aglycone class (e.g. glycoprotein-linked vs glycolipid-linked)
1.1.1  more specific aglycone class (e.g. N-glycan  vs O-glycan for proteins)</obo:UPHENO_0002032>
        <obo:IAO_0000115>A change in the strucutre of a glycan chain due to variations in the number of sugar residue constituents.</obo:IAO_0000115>
    </owl:Class>
    


    <!-- http://purl.obolibrary.org/obo/UPHENO_0002042 -->

    <owl:Class rdf:about="http://purl.obolibrary.org/obo/UPHENO_0002042">
        <rdfs:label xml:lang="en">abnormal glycan linkage</rdfs:label>
        <rdfs:subClassOf rdf:resource="http://purl.obolibrary.org/obo/UPHENO_0002004"/>
        <obo:UPHENO_0002032>Relevant Classification Axes (in order shown for exemplar classes above):
1  attachment (conjugated vs free glycans)
1.1  aglycone class (e.g. glycoprotein-linked vs glycopeptide-linked)
1.1.1  more specific aglycone class (e.g. N-glycan  vs O-glycan for proteins)</obo:UPHENO_0002032>
        <obo:IAO_0000115>A change in the strucutre of a glycan chain due to altered types of linkages between sugar residues. </obo:IAO_0000115>
    </owl:Class>
    


    <!-- http://purl.obolibrary.org/obo/UPHENO_0002043 -->

    <owl:Class rdf:about="http://purl.obolibrary.org/obo/UPHENO_0002043">
        <rdfs:label xml:lang="en">abnormal conjugated glycan composition</rdfs:label>
        <rdfs:subClassOf rdf:resource="http://purl.obolibrary.org/obo/UPHENO_0002011"/>
        <obo:IAO_0000115>A change in the strucutre of a conjugated glycan chain due to variations in number and/or type of sugar residue constituents - typically an increased or decreased abundance of a given type of residue, or the substitution of on residue type for another.</obo:IAO_0000115>
    </owl:Class>
    


    <!-- http://purl.obolibrary.org/obo/UPHENO_0002044 -->

    <owl:Class rdf:about="http://purl.obolibrary.org/obo/UPHENO_0002044">
        <rdfs:label xml:lang="en">abnormal glycoprotein glycan composition</rdfs:label>
        <rdfs:subClassOf rdf:resource="http://purl.obolibrary.org/obo/UPHENO_0002043"/>
        <obo:IAO_0000115>A change in the strucutre of a glycoprotein glycan chain due to variations in number and/or type of sugar residue constituents - typically an increased or decreased abundance of a given type of residue, or the substitution of on residue type for another.</obo:IAO_0000115>
    </owl:Class>
    


    <!-- http://purl.obolibrary.org/obo/UPHENO_0002045 -->

    <owl:Class rdf:about="http://purl.obolibrary.org/obo/UPHENO_0002045">
        <rdfs:label xml:lang="en">abnormal terminal sialyl content in N-glycans</rdfs:label>
        <rdfs:subClassOf rdf:resource="http://purl.obolibrary.org/obo/UPHENO_0002021"/>
        <obo:IAO_0000115>A change in the strucutre of an N-glycan chain due to variations in number and/or location of sialyl residues at a terminal location of a glycan chain.</obo:IAO_0000115>
    </owl:Class>
    


    <!-- http://purl.obolibrary.org/obo/UPHENO_0002046 -->

    <owl:Class rdf:about="http://purl.obolibrary.org/obo/UPHENO_0002046">
        <rdfs:label xml:lang="en">abnormal O-glycan composition</rdfs:label>
        <rdfs:subClassOf rdf:resource="http://purl.obolibrary.org/obo/UPHENO_0002044"/>
        <obo:IAO_0000115>A change in the strucutre of an O-glycan chain due to variations in number and/or type of sugar residue constituents - typically an increased or decreased abundance of a given type of residue, or the substitution of on residue type for another.</obo:IAO_0000115>
    </owl:Class>
    


    <!-- http://purl.obolibrary.org/obo/UPHENO_0002047 -->

    <owl:Class rdf:about="http://purl.obolibrary.org/obo/UPHENO_0002047">
        <rdfs:label xml:lang="en">abnormal mannosyl content in N-glycans</rdfs:label>
        <rdfs:subClassOf rdf:resource="http://purl.obolibrary.org/obo/UPHENO_0002020"/>
        <obo:IAO_0000115>A change in the strucutre of an N-glycan chain due to variations in number and/or location of mannosyl residues - typically an increased or decreased abundance of mannosyl residues, or the substitution of mannosyl residues for another residue type.</obo:IAO_0000115>
    </owl:Class>
    


    <!-- http://purl.obolibrary.org/obo/UPHENO_0002048 -->

    <owl:Class rdf:about="http://purl.obolibrary.org/obo/UPHENO_0002048">
        <rdfs:label xml:lang="en">abnormal sialyl content in serum N-glycans</rdfs:label>
        <rdfs:subClassOf rdf:resource="http://purl.obolibrary.org/obo/UPHENO_0002021"/>
        <obo:IAO_0000115>A change in the strucutre of a serum-localized N-glycan chain due to variations in number and/or location of sialyl residues - typically an increased or decreased abundance of sialyl residues, or the substitution of sialyl residues for another residue type.</obo:IAO_0000115>
    </owl:Class>
    


    <!-- http://purl.obolibrary.org/obo/UPHENO_0002049 -->

    <owl:Class rdf:about="http://purl.obolibrary.org/obo/UPHENO_0002049">
        <rdfs:label xml:lang="en">abnormal free glycan composition</rdfs:label>
        <rdfs:subClassOf rdf:resource="http://purl.obolibrary.org/obo/UPHENO_0002011"/>
        <obo:IAO_0000115>A change in the strucutre of a free glycan chain due to variations in number and/or type of sugar residue constituents - typically an increased or decreased abundance of a given type of residue, or the substitution of on residue type for another.</obo:IAO_0000115>
    </owl:Class>
    


    <!-- http://purl.obolibrary.org/obo/UPHENO_0002050 -->

    <owl:Class rdf:about="http://purl.obolibrary.org/obo/UPHENO_0002050">
        <rdfs:label xml:lang="en">abnormal glycolipid glycan composition</rdfs:label>
        <rdfs:subClassOf rdf:resource="http://purl.obolibrary.org/obo/UPHENO_0002043"/>
        <obo:IAO_0000115>A change in the strucutre of a glycolipid glycan chain due to variations in number and/or type of sugar residue constituents - typically an increased or decreased abundance of a given type of residue, or the substitution of on residue type for another.</obo:IAO_0000115>
    </owl:Class>
    


    <!-- http://purl.obolibrary.org/obo/UPHENO_0002051 -->

    <owl:Class rdf:about="http://purl.obolibrary.org/obo/UPHENO_0002051">
        <rdfs:label xml:lang="en">abnormal glycosphingolipid glycan composition</rdfs:label>
        <rdfs:subClassOf rdf:resource="http://purl.obolibrary.org/obo/UPHENO_0002050"/>
    </owl:Class>
    


    <!-- http://purl.obolibrary.org/obo/UPHENO_0002052 -->

    <owl:Class rdf:about="http://purl.obolibrary.org/obo/UPHENO_0002052">
        <rdfs:label xml:lang="en">abnormal glycoglycerolipid glycan composition</rdfs:label>
        <rdfs:subClassOf rdf:resource="http://purl.obolibrary.org/obo/UPHENO_0002050"/>
    </owl:Class>
    


    <!-- http://purl.obolibrary.org/obo/UPHENO_0002053 -->

    <owl:Class rdf:about="http://purl.obolibrary.org/obo/UPHENO_0002053">
        <rdfs:label xml:lang="en">abnormal lipopolysaccharide glycan composition</rdfs:label>
        <rdfs:subClassOf rdf:resource="http://purl.obolibrary.org/obo/UPHENO_0002043"/>
        <obo:IAO_0000115>A change in the strucutre of a lipopolysaccharide glycan chain due to variations in number and/or type of sugar residue constituents - typically an increased or decreased abundance of a given type of residue, or the substitution of on residue type for another.</obo:IAO_0000115>
    </owl:Class>
    


    <!-- http://purl.obolibrary.org/obo/UPHENO_0002054 -->

    <owl:Class rdf:about="http://purl.obolibrary.org/obo/UPHENO_0002054">
        <rdfs:label xml:lang="en">abnormal conjugated glycan length</rdfs:label>
        <rdfs:subClassOf rdf:resource="http://purl.obolibrary.org/obo/UPHENO_0002041"/>
    </owl:Class>
    


    <!-- http://purl.obolibrary.org/obo/UPHENO_0002055 -->

    <owl:Class rdf:about="http://purl.obolibrary.org/obo/UPHENO_0002055">
        <rdfs:label xml:lang="en">abnormal free glycan length</rdfs:label>
        <rdfs:subClassOf rdf:resource="http://purl.obolibrary.org/obo/UPHENO_0002041"/>
    </owl:Class>
    


    <!-- http://purl.obolibrary.org/obo/UPHENO_0002056 -->

    <owl:Class rdf:about="http://purl.obolibrary.org/obo/UPHENO_0002056">
        <rdfs:label xml:lang="en">abnormal glycoprotein glycan length</rdfs:label>
        <rdfs:subClassOf rdf:resource="http://purl.obolibrary.org/obo/UPHENO_0002054"/>
    </owl:Class>
    


    <!-- http://purl.obolibrary.org/obo/UPHENO_0002057 -->

    <owl:Class rdf:about="http://purl.obolibrary.org/obo/UPHENO_0002057">
        <rdfs:label xml:lang="en">abnormal glycolipid length</rdfs:label>
        <rdfs:subClassOf rdf:resource="http://purl.obolibrary.org/obo/UPHENO_0002054"/>
    </owl:Class>
    


    <!-- http://purl.obolibrary.org/obo/UPHENO_0002058 -->

    <owl:Class rdf:about="http://purl.obolibrary.org/obo/UPHENO_0002058">
        <rdfs:label xml:lang="en">abnormal lipopolysaccharide length</rdfs:label>
        <rdfs:subClassOf rdf:resource="http://purl.obolibrary.org/obo/UPHENO_0002054"/>
    </owl:Class>
    


    <!-- http://purl.obolibrary.org/obo/UPHENO_0002059 -->

    <owl:Class rdf:about="http://purl.obolibrary.org/obo/UPHENO_0002059">
        <rdfs:label xml:lang="en">abnormal N-glycan length</rdfs:label>
        <rdfs:subClassOf rdf:resource="http://purl.obolibrary.org/obo/UPHENO_0002056"/>
    </owl:Class>
    


    <!-- http://purl.obolibrary.org/obo/UPHENO_0002060 -->

    <owl:Class rdf:about="http://purl.obolibrary.org/obo/UPHENO_0002060">
        <rdfs:label xml:lang="en">abnormal O-glycan length</rdfs:label>
        <rdfs:subClassOf rdf:resource="http://purl.obolibrary.org/obo/UPHENO_0002056"/>
    </owl:Class>
    


    <!-- http://purl.obolibrary.org/obo/UPHENO_0002061 -->

    <owl:Class rdf:about="http://purl.obolibrary.org/obo/UPHENO_0002061">
        <rdfs:label xml:lang="en">abnormal glycopeptide glycan composition</rdfs:label>
        <rdfs:subClassOf rdf:resource="http://purl.obolibrary.org/obo/UPHENO_0002043"/>
        <obo:IAO_0000115>A change in the strucutre of a glycopeptide glycan chain due to variations in number and/or type of sugar residue constituents - typically an increased or decreased abundance of a given type of residue, or the substitution of on residue type for another.</obo:IAO_0000115>
    </owl:Class>
    


    <!-- http://purl.obolibrary.org/obo/UPHENO_0002062 -->

    <owl:Class rdf:about="http://purl.obolibrary.org/obo/UPHENO_0002062">
        <rdfs:label xml:lang="en">abnormal glycopeptide length</rdfs:label>
        <rdfs:subClassOf rdf:resource="http://purl.obolibrary.org/obo/UPHENO_0002054"/>
    </owl:Class>
    


    <!-- http://purl.obolibrary.org/obo/UPHENO_0002064 -->

    <owl:Class rdf:about="http://purl.obolibrary.org/obo/UPHENO_0002064">
        <rdfs:label xml:lang="en">abnormal conjugated glycan branching</rdfs:label>
        <rdfs:subClassOf rdf:resource="http://purl.obolibrary.org/obo/UPHENO_0002010"/>
        <obo:IAO_0000115>A change in the structure of a conjugated glycan chain due to altered branching patterns. </obo:IAO_0000115>
    </owl:Class>
    


    <!-- http://purl.obolibrary.org/obo/UPHENO_0002065 -->

    <owl:Class rdf:about="http://purl.obolibrary.org/obo/UPHENO_0002065">
        <rdfs:label xml:lang="en">abnormal free glycan branching</rdfs:label>
        <rdfs:subClassOf rdf:resource="http://purl.obolibrary.org/obo/UPHENO_0002010"/>
        <obo:IAO_0000115>A change in the structure of a free glycan chain due to altered branching patterns. </obo:IAO_0000115>
    </owl:Class>
    


    <!-- http://purl.obolibrary.org/obo/UPHENO_0002066 -->

    <owl:Class rdf:about="http://purl.obolibrary.org/obo/UPHENO_0002066">
        <rdfs:label xml:lang="en">abnormal glycoprotein glycan branching</rdfs:label>
        <rdfs:subClassOf rdf:resource="http://purl.obolibrary.org/obo/UPHENO_0002064"/>
        <obo:IAO_0000115>A change in the structure of a glycoprotein glycan chain due to altered branching patterns. </obo:IAO_0000115>
    </owl:Class>
    


    <!-- http://purl.obolibrary.org/obo/UPHENO_0002067 -->

    <owl:Class rdf:about="http://purl.obolibrary.org/obo/UPHENO_0002067">
        <rdfs:label xml:lang="en">abnormal glycopeptide glycan branching</rdfs:label>
        <rdfs:subClassOf rdf:resource="http://purl.obolibrary.org/obo/UPHENO_0002064"/>
        <obo:IAO_0000115>A change in the structure of a glycopeptide glycan chain due to altered branching patterns. </obo:IAO_0000115>
    </owl:Class>
    


    <!-- http://purl.obolibrary.org/obo/UPHENO_0002068 -->

    <owl:Class rdf:about="http://purl.obolibrary.org/obo/UPHENO_0002068">
        <rdfs:label xml:lang="en">abnormal free glycan linkage</rdfs:label>
        <rdfs:subClassOf rdf:resource="http://purl.obolibrary.org/obo/UPHENO_0002042"/>
        <obo:IAO_0000115>A change in the strucutre of a free glycan chain due to altered types of linkages between sugar residues. </obo:IAO_0000115>
    </owl:Class>
    


    <!-- http://purl.obolibrary.org/obo/UPHENO_0002069 -->

    <owl:Class rdf:about="http://purl.obolibrary.org/obo/UPHENO_0002069">
        <rdfs:label xml:lang="en">abnormal conjugated glycan linkage</rdfs:label>
        <rdfs:subClassOf rdf:resource="http://purl.obolibrary.org/obo/UPHENO_0002042"/>
        <obo:IAO_0000115>A change in the strucutre of a conjugated glycan chain due to altered types of linkages between sugar residues. </obo:IAO_0000115>
    </owl:Class>
    


    <!-- http://purl.obolibrary.org/obo/UPHENO_0002070 -->

    <owl:Class rdf:about="http://purl.obolibrary.org/obo/UPHENO_0002070">
        <rdfs:label xml:lang="en">abnormal glycoprotein glycan linkage</rdfs:label>
        <rdfs:subClassOf rdf:resource="http://purl.obolibrary.org/obo/UPHENO_0002069"/>
        <obo:IAO_0000115>A change in the strucutre of a glycoprotein glycan chain due to altered types of linkages between sugar residues. </obo:IAO_0000115>
    </owl:Class>
    


    <!-- http://purl.obolibrary.org/obo/UPHENO_0002071 -->

    <owl:Class rdf:about="http://purl.obolibrary.org/obo/UPHENO_0002071">
        <rdfs:label xml:lang="en">abnormal glycopeptide glycan linkage</rdfs:label>
        <rdfs:subClassOf rdf:resource="http://purl.obolibrary.org/obo/UPHENO_0002069"/>
        <obo:IAO_0000115>A change in the strucutre of a glycopeptide glycan chain due to altered types of linkages between sugar residues. </obo:IAO_0000115>
    </owl:Class>
    


    <!-- http://purl.obolibrary.org/obo/UPHENO_0002072 -->

    <owl:Class rdf:about="http://purl.obolibrary.org/obo/UPHENO_0002072">
        <rdfs:label xml:lang="en">abnormal O-glycan branching</rdfs:label>
        <rdfs:subClassOf rdf:resource="http://purl.obolibrary.org/obo/UPHENO_0002066"/>
        <obo:IAO_0000115>A change in the structure of an O-glycan chain due to altered branching patterns. </obo:IAO_0000115>
    </owl:Class>
    


    <!-- http://purl.obolibrary.org/obo/UPHENO_0002073 -->

    <owl:Class rdf:about="http://purl.obolibrary.org/obo/UPHENO_0002073">
        <rdfs:label xml:lang="en">abnormal O-glycan linkage</rdfs:label>
        <rdfs:subClassOf rdf:resource="http://purl.obolibrary.org/obo/UPHENO_0002070"/>
        <obo:IAO_0000115>A change in the strucutre of an O-glycan chain due to altered types of linkages between sugar residues. </obo:IAO_0000115>
    </owl:Class>
    


    <!-- http://purl.obolibrary.org/obo/UPHENO_0002074 -->

    <owl:Class rdf:about="http://purl.obolibrary.org/obo/UPHENO_0002074">
        <rdfs:label xml:lang="en">abnormal N-glycan linkage</rdfs:label>
        <rdfs:subClassOf rdf:resource="http://purl.obolibrary.org/obo/UPHENO_0002070"/>
        <obo:IAO_0000115>A change in the strucutre of n N-glycan chain due to altered types of linkages between sugar residues. </obo:IAO_0000115>
    </owl:Class>
    


    <!-- http://purl.obolibrary.org/obo/UPHENO_0002075 -->

    <owl:Class rdf:about="http://purl.obolibrary.org/obo/UPHENO_0002075">
        <rdfs:label xml:lang="en">abnormal conjugated glycan levels</rdfs:label>
        <rdfs:subClassOf rdf:resource="http://purl.obolibrary.org/obo/UPHENO_0002002"/>
        <obo:IAO_0000115>An increase or decrease in the amount or concentration of normal conjugated gycan structures present in the body, cell, or specific location therein.</obo:IAO_0000115>
    </owl:Class>
    


    <!-- http://purl.obolibrary.org/obo/UPHENO_0002076 -->

    <owl:Class rdf:about="http://purl.obolibrary.org/obo/UPHENO_0002076">
        <rdfs:label xml:lang="en">abnormal free glycan levels</rdfs:label>
        <rdfs:subClassOf rdf:resource="http://purl.obolibrary.org/obo/UPHENO_0002002"/>
        <rdfs:comment>&apos;Natively free&apos; glycans are those that are not conjugated to an aglycone target.  Many glycan assays measure glycans that have been experimentally cleaved from their aglycone target, but these are not &apos;natively&apos; free because they existed in a conjugated state in the body prior to the experiment.</rdfs:comment>
        <obo:IAO_0000115>An increase or decrease in the amount or concentration of normal, natively free glycan structures present in the body, cell, or specific location therein.</obo:IAO_0000115>
    </owl:Class>
    


    <!-- http://purl.obolibrary.org/obo/UPHENO_0002077 -->

    <owl:Class rdf:about="http://purl.obolibrary.org/obo/UPHENO_0002077">
        <rdfs:label xml:lang="en">abnormal glycoprotein glycan levels</rdfs:label>
        <rdfs:subClassOf rdf:resource="http://purl.obolibrary.org/obo/UPHENO_0002075"/>
        <obo:IAO_0000115>An increase or decrease in the amount or concentration of normal glycoprotein gycan structures present in the body, cell, or specific location therein.</obo:IAO_0000115>
    </owl:Class>
    


    <!-- http://purl.obolibrary.org/obo/UPHENO_0002078 -->

    <owl:Class rdf:about="http://purl.obolibrary.org/obo/UPHENO_0002078">
        <rdfs:label xml:lang="en">abnormal glycopeptide glycan levels</rdfs:label>
        <rdfs:subClassOf rdf:resource="http://purl.obolibrary.org/obo/UPHENO_0002075"/>
        <obo:IAO_0000115>An increase or decrease in the amount or concentration of normal glycopeptide gycan structures present in the body, cell, or specific location therein.</obo:IAO_0000115>
    </owl:Class>
    


    <!-- http://purl.obolibrary.org/obo/UPHENO_0002079 -->

    <owl:Class rdf:about="http://purl.obolibrary.org/obo/UPHENO_0002079">
        <rdfs:label xml:lang="en">abnormal glycolipid levels</rdfs:label>
        <rdfs:subClassOf rdf:resource="http://purl.obolibrary.org/obo/UPHENO_0002075"/>
        <obo:IAO_0000115>An increase or decrease in the amount or concentration of normal glycolipid gycan structures present in the body, cell, or specific location therein.</obo:IAO_0000115>
    </owl:Class>
    


    <!-- http://purl.obolibrary.org/obo/UPHENO_0002081 -->

    <owl:Class rdf:about="http://purl.obolibrary.org/obo/UPHENO_0002081">
        <rdfs:label xml:lang="en">abnormal glycosaminoglycan length</rdfs:label>
        <rdfs:subClassOf rdf:resource="http://purl.obolibrary.org/obo/UPHENO_0002056"/>
    </owl:Class>
    


    <!-- http://purl.obolibrary.org/obo/UPHENO_0002082 -->

    <owl:Class rdf:about="http://purl.obolibrary.org/obo/UPHENO_0002082">
        <rdfs:label xml:lang="en">abnormal intracellular free glycan levels</rdfs:label>
        <rdfs:subClassOf rdf:resource="http://purl.obolibrary.org/obo/UPHENO_0002076"/>
        <obo:IAO_0000115>An increase or decrease in the amount or concentration of normal free gycan structures present in the intracellular space.</obo:IAO_0000115>
    </owl:Class>
    


    <!-- http://purl.obolibrary.org/obo/UPHENO_0002083 -->

    <owl:Class rdf:about="http://purl.obolibrary.org/obo/UPHENO_0002083">
        <rdfs:label xml:lang="en">abnormal extracellular free glycan levels</rdfs:label>
        <rdfs:subClassOf rdf:resource="http://purl.obolibrary.org/obo/UPHENO_0002076"/>
        <obo:IAO_0000115>An increase or decrease in the amount or concentration of normal, natively free gycan structures present in the extracellular space.</obo:IAO_0000115>
    </owl:Class>
    


    <!-- http://purl.obolibrary.org/obo/UPHENO_0002084 -->

    <owl:Class rdf:about="http://purl.obolibrary.org/obo/UPHENO_0002084">
        <rdfs:label xml:lang="en">abnormal free glycan levels in urine</rdfs:label>
        <rdfs:subClassOf rdf:resource="http://purl.obolibrary.org/obo/UPHENO_0002083"/>
        <obo:IAO_0000115>An increase or decrease in the amount or concentration of normal, natively free gycan structures present in the urine..</obo:IAO_0000115>
    </owl:Class>
    


    <!-- http://purl.obolibrary.org/obo/UPHENO_0002085 -->

    <owl:Class rdf:about="http://purl.obolibrary.org/obo/UPHENO_0002085">
        <rdfs:label xml:lang="en">abnormal free glycan levels in serum</rdfs:label>
        <rdfs:subClassOf rdf:resource="http://purl.obolibrary.org/obo/UPHENO_0002083"/>
        <obo:IAO_0000115>An increase or decrease in the amount or concentration of normal, natively free gycan structures present in the blood serum..</obo:IAO_0000115>
    </owl:Class>
    


    <!-- http://purl.obolibrary.org/obo/UPHENO_0002086 -->

    <owl:Class rdf:about="http://purl.obolibrary.org/obo/UPHENO_0002086">
        <rdfs:label xml:lang="en">abnormal free glycan levels in CSF</rdfs:label>
        <rdfs:subClassOf rdf:resource="http://purl.obolibrary.org/obo/UPHENO_0002083"/>
        <obo:IAO_0000115>An increase or decrease in the amount or concentration of normal, natively free gycan structures present in the CSF fluid.</obo:IAO_0000115>
    </owl:Class>
    


    <!-- http://purl.obolibrary.org/obo/UPHENO_0002087 -->

    <owl:Class rdf:about="http://purl.obolibrary.org/obo/UPHENO_0002087">
        <rdfs:label xml:lang="en">abnormal GPI-anchor glycan levels</rdfs:label>
        <rdfs:subClassOf rdf:resource="http://purl.obolibrary.org/obo/UPHENO_0002077"/>
        <obo:IAO_0000115>An increase or decrease in the amount or concentration of normal GPI-anchored gycan structures present in the body, cell, or specific location therein.</obo:IAO_0000115>
    </owl:Class>
    


    <!-- http://purl.obolibrary.org/obo/UPHENO_0002088 -->

    <owl:Class rdf:about="http://purl.obolibrary.org/obo/UPHENO_0002088">
        <rdfs:label xml:lang="en">abnormal glycosphingomyelin glycan levels</rdfs:label>
        <rdfs:subClassOf rdf:resource="http://purl.obolibrary.org/obo/UPHENO_0002079"/>
        <obo:IAO_0000115>An increase or decrease in the amount or concentration of normal glycosphingomyelin gycan structures present in the body, cell, or specific location therein.</obo:IAO_0000115>
    </owl:Class>
    


    <!-- http://purl.obolibrary.org/obo/UPHENO_0002089 -->

    <owl:Class rdf:about="http://purl.obolibrary.org/obo/UPHENO_0002089">
        <rdfs:label xml:lang="en">abnormal glycoglycerolipid levels</rdfs:label>
        <rdfs:subClassOf rdf:resource="http://purl.obolibrary.org/obo/UPHENO_0002079"/>
        <obo:IAO_0000115>An increase or decrease in the amount or concentration of normal glycoglycerolipid gycan structures present in the body, cell, or specific location therein.</obo:IAO_0000115>
    </owl:Class>
    


    <!-- http://purl.obolibrary.org/obo/UPHENO_0002090 -->

    <owl:Class rdf:about="http://purl.obolibrary.org/obo/UPHENO_0002090">
        <rdfs:label xml:lang="en">abnormal lipopolysaccharide glycan levels</rdfs:label>
        <rdfs:subClassOf rdf:resource="http://purl.obolibrary.org/obo/UPHENO_0002075"/>
        <obo:IAO_0000115>An increase or decrease in the amount or concentration of normal lipopolysaccharide gycan structures present in the body, cell, or specific location therein.</obo:IAO_0000115>
    </owl:Class>
    


    <!-- http://purl.obolibrary.org/obo/UPHENO_0002091 -->

    <owl:Class rdf:about="http://purl.obolibrary.org/obo/UPHENO_0002091">
        <rdfs:label xml:lang="en">abnormal oligomannose N-glycan levels</rdfs:label>
        <rdfs:subClassOf rdf:resource="http://purl.obolibrary.org/obo/UPHENO_0002014"/>
        <obo:IAO_0000115>An increase or decrease in the amount or concentration of normal oligomannose N-gycan structures present in the body, cell, or specific location therein.</obo:IAO_0000115>
    </owl:Class>
    


    <!-- http://purl.obolibrary.org/obo/UPHENO_0002092 -->

    <owl:Class rdf:about="http://purl.obolibrary.org/obo/UPHENO_0002092">
        <rdfs:label xml:lang="en">abnormal Man9GlcNAc2 glycan levels</rdfs:label>
        <rdfs:subClassOf rdf:resource="http://purl.obolibrary.org/obo/UPHENO_0002091"/>
        <obo:IAO_0000115>An increase or decrease in the amount or concentration of Man9GlcNAc2 gycan structures present in the body, cell, or specific location therein.</obo:IAO_0000115>
    </owl:Class>
    


    <!-- http://purl.obolibrary.org/obo/UPHENO_0002093 -->

    <owl:Class rdf:about="http://purl.obolibrary.org/obo/UPHENO_0002093">
        <rdfs:label xml:lang="en">abnormal oligomannose N-glycan levels in golgi</rdfs:label>
        <rdfs:subClassOf rdf:resource="http://purl.obolibrary.org/obo/UPHENO_0002091"/>
        <obo:IAO_0000115>An increase or decrease in the amount or concentration of normal oligomannose N-gycan structures present in the golgi complex.</obo:IAO_0000115>
    </owl:Class>
    


    <!-- http://purl.obolibrary.org/obo/UPHENO_0002094 -->

    <owl:Class rdf:about="http://purl.obolibrary.org/obo/UPHENO_0002094">
        <rdfs:label xml:lang="en">abnormal transferrin-linked oligomannose N-glycan levels</rdfs:label>
        <rdfs:subClassOf rdf:resource="http://purl.obolibrary.org/obo/UPHENO_0002091"/>
        <obo:IAO_0000115>An increase or decrease in the amount or concentration of transferring-linked oligomannose N-gycan structures present in the body, cell, or specific location therein.</obo:IAO_0000115>
    </owl:Class>
    


    <!-- http://purl.obolibrary.org/obo/UPHENO_0002095 -->

    <owl:Class rdf:about="http://purl.obolibrary.org/obo/UPHENO_0002095">
        <rdfs:label xml:lang="en">abnormal Tn core O-glycan levels</rdfs:label>
        <rdfs:subClassOf rdf:resource="http://purl.obolibrary.org/obo/UPHENO_0002015"/>
        <obo:IAO_0000115>An increase or decrease in the amount or concentration of Tn core O-gycan structures present in the body, cell, or specific location therein.</obo:IAO_0000115>
    </owl:Class>
    


    <!-- http://purl.obolibrary.org/obo/UPHENO_0002096 -->

    <owl:Class rdf:about="http://purl.obolibrary.org/obo/UPHENO_0002096">
        <rdfs:label xml:lang="en">abnormal Tn core O-glycan levels in blood cell plasma membrane</rdfs:label>
        <rdfs:subClassOf rdf:resource="http://purl.obolibrary.org/obo/UPHENO_0002095"/>
        <obo:IAO_0000115>An increase or decrease in the amount or concentration of Tn core O-gycan structures present in the plasma membrane of blood cells.</obo:IAO_0000115>
    </owl:Class>
</rdf:RDF>



<!-- Generated by the OWL API (version 3.4.2) http://owlapi.sourceforge.net -->

